Typing checking statements in the new style. We also no longer pretend that the list of identifiers bound in a block form an environment (because our implementation of environments happes to be list-based) so there's more to check (e.g. no duplicates).

ott/coq/Context.v
@@ -3,19 +3,34 @@ Require Import Common.
 Definition context (A B : Set) := list (A * B).
 Arguments context : default implicits.
 
+Definition empty {A B : Set} : context A B := nil.
+
 Definition eq_context {A B} eq_A eq_B : context A B -> context A B -> bool :=
   eq_list (eq_pair eq_A eq_B).
 
-Definition add {A B} (C : context A B) a b :=
+Definition add {A B} a b (C : context A B) :=
   (a, b) :: C.
 
+Definition add_bindings {A B : Set} (bs : list (A * B)) (C : context A B) := List.fold_left (fun C b => b :: C) bs C.
+
 Definition lookup {A B : Set} (eq_A : A -> A -> bool) :=
-  fix lookup (E : context A B) (a : A) : option B :=
-    match E with
-      | nil          => None
-      | cons (x,b) E => if eq_A x a then Some b
-                                    else lookup E a
+  fix lookup (C : context A B) (a : A) : option B :=
+    match C with
+      | nil         => None
+      | (x, b) :: C => if eq_A x a then Some b
+                                   else lookup C a
     end.
+
+Definition mem {A B : Set} (eq_A : A -> A -> bool) a (C: context A B) :=
+  match lookup eq_A C a with
+  | Some _ => true
+  | None   => false
+  end.
+
+Definition fresh {A B : Set} (eq_A : A -> A -> bool) a (C: context A B) := negb (mem eq_A a C).
+
+Definition fresh_bindings {A B1 B2 : Set} (eq_A : A -> A -> bool) (bs : list (A * B2)) (C: context A B1) :=
+  all_list (fun b => fresh eq_A (fst b) C) bs.
 
 Fixpoint remove_var {A B: Set} (eq_A : A -> A -> bool) a C : context A B :=
   match C with
@@ -57,3 +72,21 @@ Definition equiv_p {A B: Set} (eq_A : A -> A -> bool) (p : A -> bool) (equiv_B :
 
 Definition equiv {A B: Set} (eq_A : A -> A -> bool) (equiv_B : B -> B -> bool)  (C1 C2 : context A B) :=
   sub eq_A equiv_B C1 C2 && sub eq_A equiv_B C2 C1.
+
+Fixpoint disjoint {A B1 B2} eq_A (C1 : context A B1) (C2 : context A B2) : bool :=
+  match C1 with
+  | nil          => true
+  | (a, _) :: C1 => match lookup eq_A C2 a with
+                    | Some _ => false
+                    | None   => disjoint eq_A C1 C2
+                    end
+  end.
+
+Definition fresh_in_bindings {A B : Set} eq_A (a : A) (xs : list (A * B)) :=
+  all_list (fun x => negb (eq_A a (fst x))) xs.
+
+Fixpoint disjoint_bindings {A B : Set} eq_A (xs : list (A * B)) :=
+  match xs with
+  | (a, _) :: xs => fresh_in_bindings eq_A a xs && disjoint_bindings eq_A xs
+  | nil          => true
+  end.
