ott/coq/Context_defns.v
@@ -5,8 +5,14 @@ Inductive lookup {A B : Set} : context A B -> A -> B -> Type :=
   | Lookup_hd     a b C :                           lookup ((a,b) :: C) a b
   | Lookup_tl x y a b C : x <> a -> lookup C a b -> lookup ((x,y) :: C) a b.
 
-Definition disjoint {A B1 B2 : Set} C1 C2 : Type :=
-  forall (a : A) (b1 : B1) (b2 : B2), lookup C1 a b1 -> lookup C2 a b2 -> False.
+Definition mem {A B} a (C : context A B) := {b : B & lookup C a b}.
+
+Definition fresh {A B} a (C : context A B) := neg (mem a C).
+
+Definition freshBindings {A B1 B2 : Set} (bs : list (A * B1)) (C : context A B2) := allList (fun b => fresh (fst b) C) bs.
+
+Definition disjoint {A B1 B2 : Set} (C1 : context A B1) (C2 : context A B2) : Type :=
+  forall (a : A), mem a C1 -> mem a C2 -> False.
 
 Definition subP {A B: Set} (P : A -> Type) (E : B -> B -> Type) (C1 C2 : context A B) :=
   forall id, P id -> forall b1, lookup C1 id b1 -> {b2 : B & lookup C2 id b2 * E b1 b2}.
@@ -22,4 +28,20 @@ Definition equiv {A B: Set} (E : B -> B -> Type) (C1 C2 : context A B) :=
 
 Inductive linear {A B: Set} : context A B -> Type :=
   | Linear_nil        : linear nil
-  | Linear_cons a b C : (forall b, neg (lookup C a b)) -> linear C -> linear (add C a b).
+  | Linear_cons a b C : (forall b, neg (lookup C a b)) -> linear C -> linear (add a b C).
+
+Inductive freshInBindings {A B : Set} : A -> list (A * B) -> Prop :=
+ | FreshInBindings_nil a' :
+     freshInBindings a' nil
+ | FreshInBindings_cons a' a b bs :
+     neg (a' = a) ->
+     freshInBindings a' bs ->
+     freshInBindings a' ((a, b) :: bs).
+
+Inductive disjointBindings {A B : Set} : list (A * B) -> Prop :=
+ | DisjointBindings_nil :
+     disjointBindings nil
+ | DisjointBindings_cons a b xs :
+     freshInBindings a xs ->
+     disjointBindings xs ->
+     disjointBindings ((a, b) :: xs).
